\section{Crout Factorization}
	
	\begin{align}
		A &= \begin{bmatrix}
				1 & -1 & 0 \\[0.3em]
				-2 & 4 & -2 \\[0.3em]
				0 & -1 & 2
			\end{bmatrix}&
	\label{eq:52}
	\end{align}

	Starting defining the Crout Factorization of \cref{eq:52}:

	\begin{align}
		A &= \begin{bmatrix}
				1 & -1 & 0 \\[0.3em]
				-2 & 4 & -2 \\[0.3em]
				0 & -1 & 2
			\end{bmatrix}
			=
			\begin{bmatrix}
				l_{11} & 0 & 0 \\[0.3em]
				l_{21} & l_{22} & 0 \\[0.3em]
				l_{31} & l_{32} & l_{33}
			\end{bmatrix}
			\begin{bmatrix}
				1 & U_{12} & U_{13} \\[0.3em]
				0 & 1 & U_{23} \\[0.3em]
				0 & 0 & 1
			\end{bmatrix}&
	\end{align}
	\begin{align}
		l_{11}U_{11} &= A_{11}& \notag \\
		l_{11}*1 &= 1& \notag \\
		&= 1&
	\end{align}
	\begin{align}
		l_{21}U_{11} &= A_{21}& \notag \\
		l_{21}*1 &= -2& \notag \\
		&= -2& \\
		l_{31}U_{11} &= A_{31}& \notag \\
		l_{31}*1 &= 0& \notag \\
		&= 0& \\
		\notag \\		
		l_{11}U_{12} &= A_{12}& \notag \\
		1*U_{12} &= -1& \notag \\
		&= -1& \\
		\notag \\
		l_{11}*U_{13} &= A_{13}& \notag \\
		1*U_{13} &= 0& \notag \\
		&= 0& \\
		\notag \\
		l_{21}U_{12} + l_{22}U_{22} &= A_{22}& \notag \\
		(-2)*(-1) + l_{22}*1 &= 4& \notag \\
		l_{22} &= 4 - 2 = 2& \\
		\notag \\
		l_{21}U_{13} + l_{22}U_{23} &= A_{23}& \notag \\
		(-2)*0 + 2*U_{23} &= -2& \notag \\
		U_{23} &= -\frac{2}{2} = -1 \\
		\notag \\
		l_{31}U_{12} + l_{32}U_{22} &= A_{32}& \notag \\
		0*(-1) + l_{32}*1 &= -1& \notag \\
		&= -1& \\
		\notag \\
		l_{31}U_{13} + l_{32}U_{23} + l_{33}U_{33} &= A_{33}& \notag \\
		(-1)*0 + (-1)*(-1) + l_{33}*1 &= 2& \notag \\
		l_{33} &= 2 - 1 = 1&
	\label{eq:52terms}
	\end{align}

	\begin{align}
		A &= \begin{bmatrix}
				1 & -1 & 0 \\[0.3em]
				-2 & 4 & -2 \\[0.3em]
				0 & -1 & 2
			\end{bmatrix}
			=
			\begin{bmatrix}
				1 & 0 & 0 \\[0.3em]
				-2 & 2 & 0 \\[0.3em]
				0 & -1 & 1
			\end{bmatrix}
			\begin{bmatrix}
				1 & -1 & 0 \\[0.3em]
				0 & 1 & -1 \\[0.3em]
				0 & 0 & 1
			\end{bmatrix}&
	\label{eq:52crout}
	\end{align}

	Solving:

	\begin{align}
		Ax &= B& \\
		Ax &= \begin{bmatrix}
				0 \\[0.3em]
				-1 \\[0.3em]
				4
			\end{bmatrix}&
	\label{eq:52ax}
	\end{align}

	Forward Substitution:

	\begin{align}
		LY &= B& \\
		\begin{bmatrix}
			1 & 0 & 0 \\[0.3em]
			-2 & 2 & 0 \\[0.3em]
			0 & -1 & 1
		\end{bmatrix}
		\begin{bmatrix}
			y_{1} \\[0.3em]
			y_{2} \\[0.3em]
			y_{3}
		\end{bmatrix} &= \begin{bmatrix}
				0 \\[0.3em]
				-1 \\[0.3em]
				4
			\end{bmatrix}& \notag \\
		\begin{bmatrix}
			y_{1} \\[0.3em]
			-2y_{1} + 2y_{2} \\[0.3em]
			-y_{2} + y_{3}
		\end{bmatrix} &= \begin{bmatrix}
				0 \\[0.3em]
				-1 \\[0.3em]
				4
			\end{bmatrix}& \notag \\
		y_{1} &= 0& \\
		y_{2} &= -\frac{1}{2}& \\
		y_{3} &= 4 - \frac{1}{2} = \frac{7}{2}&
	\label{eq:52y}
	\end{align}

	Backward Substitution:

	\begin{align}
		UX &= Y& \\
		\begin{bmatrix}
			1 & -1 & 0 \\[0.3em]
			0 & 1 & -1 \\[0.3em]
			0 & 0 & 1
		\end{bmatrix}
		\begin{bmatrix}
			x_{1} \\[0.3em]
			x_{2} \\[0.3em]
			x_{3}
		\end{bmatrix} &= \begin{bmatrix}
				0 \\[0.3em]
				-\frac{1}{2} \\[0.3em]
				\frac{7}{2}
			\end{bmatrix}& \notag \\
		\begin{bmatrix}
			x_{1} - x_{2} \\[0.3em]
			x_{2} - x_{3} \\[0.3em]
			x_{3}
		\end{bmatrix} &= \begin{bmatrix}
				0 \\[0.3em]
				-\frac{1}{2} \\[0.3em]
				\frac{7}{2}
			\end{bmatrix}& \notag \\
		x_{3} &= \frac{7}{2}& \\
		x_{2} &= -\frac{1}{2} + \frac{7}{2} = 3& \\
		x_{1} &= 3
	\label{eq:52x}
	\end{align}