\section{Approximation in a BVP using Finite Differences}

	\begin{align}
		&2xy'' + y' - 4y = x + 1&
		&y(1) = 2&
		&y(5) = 8&
		&n = 4&
	\end{align}

	\begin{align}
		&y' = \frac{y_{i+1} - y_{i-1}}{2h}&
		&y'' = \frac{y_{i+1} - 2y_{i} + y_{i-1}}{h^{2}}&
	\end{align}

	\begin{align}
		h &= \frac{b-a}{n} = \frac{5-1}{4} = 1&
		i &= 1,\dots,3&
	\end{align}

	\begin{align}
		2x_{i}
		\left(
			\frac{y_{i+1} - 2y_{i} + y_{i-1}}{h^{2}}
		\right)
		+
		\left(
			\frac{y_{i+1} - y_{i-1}}{2h}
		\right)
		- 4y_{i} &= x_{i} + 1&
	\end{align}

	\begin{align}
		i=1,x=2: \ &
		2x_{1}
		\left(
			\frac{y_{2} - 2y_{1} + y_{0}}{h^{2}}
		\right)
		+
		\left(
			\frac{y_{2} - y_{0}}{2h}
		\right)
		- 4y_{1} = x_{1} + 1&
		\\ &
		2(2)
		\left(
			\frac{y_{2} - 2y_{1} + 0}{1^{2}}
		\right)
		+
		\left(
			\frac{y_{2} - 0}{2(1)}
		\right)
		- 4y_{1} = 2 + 1&
		\notag \\ &
		4
		\left(
			y_{2} - 2y_{1}
		\right)
		+
		\frac{y_{2}}{2} - 4y_{1} = 3&
		\notag \\ &
		4y_{2} - 8y_{1} + \frac{y_{2}}{2} - 4y_{1} = 3&
		\notag \\ &
		-12y_{1} + \frac{9}{2}y_{2} = 3&
		\\
	\end{align}
	\begin{align}
		i=2,x=3: \ &
		2x_{2}
		\left(
			y_{3} - 2y_{2} + y_{1}
		\right)
		+
		\left(
			\frac{y_{3} - y_{1}}{2}
		\right)
		- 4y_{2} = x_{2} + 1&
		\\ &
		2(3)
		\left(
			y_{3} - 2y_{2} + y_{1}
		\right)
		+
		\left(
			\frac{y_{3} - y_{1}}{2}
		\right)
		- 4y_{2} = 3 + 1&
		\notag \\ &
		6
		\left(
			y_{3} - 2y_{2} + y_{1}
		\right)
		+
		\frac{y_{3}}{2} - \frac{y_{1}}{2} - 4y_{2} = 4&
		\notag \\ &
		6y_{3} - 12y_{2} + 6y_{1} + \frac{y_{3}}{2} - \frac{y_{1}}{2} - 4y_{2} = 4&
		\notag \\ &
		\frac{11}{2}y_{1} - 16y_{2} + \frac{13}{2}y_{3} = 4&
		\\
	\end{align}
	\begin{align}
		i=3,x=4: \ &
		2x_{3}
		\left(
			y_{4} - 2y_{3} + y_{2}
		\right)
		+
		\left(
			\frac{y_{4} - y_{2}}{2}
		\right)
		- 4y_{3} = x_{3} + 1&
		\\ &
		2(4)
		\left(
			8 - 2y_{3} + y_{2}
		\right)
		+
		\left(
			\frac{8 - y_{2}}{2}
		\right)
		- 4y_{3} = 4 + 1&
		\notag \\ &
		8
		\left(
			8 - 2y_{3} + y_{2}
		\right)
		+
		4 - \frac{y_{2}}{2} - 4y_{3} = 5&
		\notag \\ &
		64 - 16y_{3} + 8y_{2} + 4 - \frac{y_{2}}{2} - 4y_{3} = 5&
		\notag \\ &
		\frac{15}{2}y_{2} - 20y_{3} = -63&
	\end{align}

	\begin{align}
		\begin{bmatrix}
			-12 & \frac{9}{2} & 0 \\[0.7em]
			\frac{11}{2} & -16 & \frac{13}{2} \\[0.7em]
			0 & \frac{15}{2} & -20
		\end{bmatrix}
		\begin{bmatrix}
			y_{1} \\[0.7em]
			y_{2} \\[0.7em]
			y_{3}
		\end{bmatrix}
		=&
		\begin{bmatrix}
			3 \\[0.7em]
			4 \\[0.7em]
			-63
		\end{bmatrix}&
		\label{eq:q4_matrix}
	\end{align}

	Using \textbf{GNU Octave} to solve \cref{eq:q4_matrix}:

	\begin{align}
		\begin{bmatrix}
			y_{1} \\[0.7em]
			y_{2} \\[0.7em]
			y_{3}
		\end{bmatrix}
		=&
		\begin{bmatrix}
			0.24239 \\[0.7em]
			1.31304 \\[0.7em]
			3.64239
		\end{bmatrix}&
	\end{align}
