\section{Multiplicity of a Root}

	\begin{align}
		f(x) &= (x-1)^{2}\ln(x)& \notag \\
		f(x) &= (x^{2} - 2x + 1)\ln(x)& \notag \\
		f(x) &= x^{2}\ln(x) - 2x\ln(x) + \ln(x)&
	\label{eq:33}
	\end{align}

	Verifying if $x=1$ is a root of \cref{eq:33}:

	\begin{align}
		f(1) &= (1-1)^{2}\ln(1)& &;&
		f(1) &= 0*\ln(1) = 0&
	\label{eq:331x}
	\end{align}

	$x=1$ is a root of \cref{eq:33}, as can be seen in \cref{eq:331x}. To discover the multiplicity, it is necessary to discover how many derivates of \cref{eq:33} have $x=1$ as root:

	\begin{align}
		f(x) &= x^{2}\ln(x) - 2x\ln(x) + \ln(x)& \notag \\
		f'(x) &= 2x*\ln(x) + \frac{x^{2}}{x} -2 * \left( \ln(x) + \frac{x}{x} \right) + \frac{1}{x}& \notag \\
		f'(x) &= 2x*\ln(x) - 2\ln(x) + x  + \frac{1}{x} - 2&
	\label{eq:33derivate}
	\end{align}

	Verifying if $x=1$ is a root of \cref{eq:33derivate}:

	\begin{align}
		f'(1) &= 2*1*\ln(1) - 2*\ln(1) + 1 + \frac{1}{1} - 2& \notag \\
		f'(1) &= 0 - 0 + 1 + 1 - 2 = 0&
	\label{eq:33derivate1x}
	\end{align}

	\begin{align}
		f'(x) &= 2x*\ln(x) - 2\ln(x) + x  + \frac{1}{x} - 2& \notag \\
		f''(x) &= 2*\left(\ln(x) + \frac{x}{x}\right) - \frac{2}{x} + 1  - \frac{1}{x^2}& \notag \\
		f''(x) &= 2*\ln(x) - \frac{1}{x^2} - \frac{2}{x} + 3&
	\label{eq:332ndderivate}
	\end{align}

	Verifying if $x=1$ is a root of \cref{eq:332ndderivate}:

	\begin{align}
		f''(1) &= 2*\ln(1) - \frac{1}{1^2} - \frac{2}{1} + 3& \notag \\
		f''(1) &= 0 - 1 - 2 + 3 = 0& \notag \\
	\label{eq:332ndderivate1x}
	\end{align}

	\begin{align}
		f''(x) &= 2*\ln(x) - \frac{1}{x^2} - \frac{2}{x} + 3& \notag \\
		f'''(x) &=  \frac{1}{x^3} + \frac{2}{x^2} + \frac{2}{x}&
	\label{eq:333rdderivate}
	\end{align}

	Verifying if $x=1$ is a root of \cref{eq:333rdderivate}:

	\begin{align}
		f'''(1) &=  \frac{1}{1^3} + \frac{2}{1^2} + \frac{2}{1}& \notag \\
		f'''(1) &=  1 + 2 + 2 = 5 \neq 0&
	\label{eq:333rdderivate1x}
	\end{align}

	The multiplicity of $x = \alpha = 1$ in \cref{eq:33} is $3$.