\section{Doolittle Factorization}

	\begin{align}
		A &= \begin{bmatrix}
				8 & 5 & 1 \\[0.3em]
				3 & 7 & 4 \\[0.3em]
				2 & 3 & 9
			\end{bmatrix}&
	\label{eq:51}
	\end{align}

	Starting defining the Doolittle Factorization of \cref{eq:51}:

	\begin{align}
		A &= \begin{bmatrix}
				8 & 5 & 1 \\[0.3em]
				3 & 7 & 4 \\[0.3em]
				2 & 3 & 9
			\end{bmatrix}
			=
			\begin{bmatrix}
				1 & 0 & 0 \\[0.3em]
				l_{21} & 1 & 0 \\[0.3em]
				l_{31} & l_{32} & 1
			\end{bmatrix}
			\begin{bmatrix}
				U_{11} & U_{12} & U_{13} \\[0.3em]
				0 & U_{22} & U_{23} \\[0.3em]
				0 & 0 & U_{33}
			\end{bmatrix}&
	\end{align}
	\begin{align}
		l_{11}U_{11} &= A_{11}& \notag \\
		1*U_{11} &= 8& \notag \\
		&= 8& \\
		l_{11}U_{12} &= A_{12}& \notag \\
		1*U_{12} &= 5& \notag \\
		&= 5& \\
		l_{11}*U_{13} &= A_{13}& \notag \\
		1*U_{13} &= 1& \notag \\
		&= 1&
	\end{align}
	\begin{align}
		l_{21}U_{11} &= A_{21}& \notag \\
		l_{21}*8 &= 3& \notag \\
		l_{21} &= \frac{3}{8}& \\
		\notag \\
		l_{31}U_{11} &= A_{31}& \notag \\
		l_{31}*8 &= 2& \notag \\
		l_{31} &= \frac{2}{8} = \frac{1}{4}& \\
		\notag \\
		l_{21}U_{12} + l_{22}U_{22} &= A_{22}& \notag \\
		\frac{3}{8}*5 + 1*U_{22} &= 7& \notag \\
		U_{22} &= 7 - 5*\frac{3}{8}& \notag \\
		&= \frac{56 - 15}{8} = \frac{41}{8}& \\
		\notag \\
		\notag \\
		l_{21}U_{13} + l_{22}U_{23} &= A_{23}& \notag \\
		\frac{3}{8}*1 + 1*U_{23} &= 4& \notag \\
		U_{23} &= 4 - \frac{3}{8}& \notag \\
		&= \frac{32 - 3}{8} = \frac{29}{8}& \\
		\notag \\
		l_{31}U_{12} + l_{32}U_{22} &= A_{32}& \notag \\
		\frac{1}{4}*5 + l_{32}*\frac{41}{8} &= 3& \notag \\
		l_{32} &= \frac{3 - \frac{5}{4}}{\frac{41}{8}}& \notag \\
		&= \frac{\frac{12 - 5}{4}}{\frac{41}{8}} = \frac{7}{4}*\frac{8}{41} = \frac{56}{164} = \frac{14}{41}&
	\end{align}
	\begin{align}
		l_{31}U_{13} + l_{32}U_{23} + l_{33}U_{33} &= A_{33}& \notag \\
		\frac{1}{4}*1 + \frac{14}{41}*\frac{29}{8} + 1*U_{33} &= 9& \notag \\
		U_{33} &= 9 - \left(\frac{1}{4} + \frac{14}{41}*\frac{29}{8}\right)& \notag \\
		&= 9 - \frac{1}{4} - \frac{406}{328}& \notag \\
		&= \frac{36 - 1}{4} - \frac{203}{164}& \notag \\
		&= \frac{1435 - 203}{164} = \frac{1232}{164} = \frac{308}{41}&
	\label{eq:51terms}
	\end{align}

	\begin{align}
		A &= \begin{bmatrix}
				8 & 5 & 1 \\[0.3em]
				3 & 7 & 4 \\[0.3em]
				2 & 3 & 9
			\end{bmatrix}
			=
			\begin{bmatrix}
				1 & 0 & 0 \\[0.3em]
				\frac{3}{8} & 1 & 0 \\[0.3em]
				\frac{1}{4} & \frac{14}{41} & 1
			\end{bmatrix}
			\begin{bmatrix}
				8 & 5 & 1 \\[0.3em]
				0 & \frac{41}{8} & \frac{29}{8} \\[0.3em]
				0 & 0 & \frac{308}{41}
			\end{bmatrix}&
	\label{eq:51doolittle}
	\end{align}

	Solving:

	\begin{align}
		Ax &= B& \\
		Ax &= \begin{bmatrix}
				6 \\[0.3em]
				1 \\[0.3em]
				-2
			\end{bmatrix}&
	\label{eq:51ax}
	\end{align}

	Forward Substitution:

	\begin{align}
		LY &= B& \\
		\begin{bmatrix}
			1 & 0 & 0 \\[0.3em]
			\frac{3}{8} & 1 & 0 \\[0.3em]
			\frac{1}{4} & \frac{14}{41} & 1
		\end{bmatrix}
		\begin{bmatrix}
			y_{1} \\[0.3em]
			y_{2} \\[0.3em]
			y_{3}
		\end{bmatrix} &= \begin{bmatrix}
				6 \\[0.3em]
				1 \\[0.3em]
				-2
			\end{bmatrix}& \notag \\
		\begin{bmatrix}
			y_{1} \\[0.3em]
			\frac{3}{8}y_{1} + y_{2} \\[0.3em]
			\frac{1}{4}y_{1} + \frac{14}{41}y_{2} + y_{3}
		\end{bmatrix} &= \begin{bmatrix}
				6 \\[0.3em]
				1 \\[0.3em]
				-2
			\end{bmatrix}& \notag \\
		y_{1} &= 6& \\
		y_{2} &= 1 - \frac{9}{4} = - \frac{5}{4}& \\
		y_{3} &= - 2 - \frac{3}{2} + \frac{70}{164}& \notag \\
		&= - \frac{7}{2} + \frac{35}{82} = \frac{35-287}{82} = -\frac{252}{82} = -\frac{126}{41}&
	\label{eq:51y}
	\end{align}

	Backward Substitution:

	\begin{align}
		UX &= Y& \\
		\begin{bmatrix}
			8 & 5 & 1 \\[0.3em]
			0 & \frac{41}{8} & \frac{29}{8} \\[0.3em]
			0 & 0 & \frac{308}{41}
		\end{bmatrix}
		\begin{bmatrix}
			x_{1} \\[0.3em]
			x_{2} \\[0.3em]
			x_{3}
		\end{bmatrix} &= \begin{bmatrix}
				6 \\[0.3em]
				-\frac{5}{4} \\[0.3em]
				-\frac{126}{41}
			\end{bmatrix}& \notag \\
		\begin{bmatrix}
			8x_{1} + 5x_{2} + x_{3} \\[0.3em]
			\frac{41}{8}x_{2} + \frac{29}{8}x_{3} \\[0.3em]
			\frac{308}{41}x_{3}
		\end{bmatrix} &= \begin{bmatrix}
				6 \\[0.3em]
				-\frac{5}{4} \\[0.3em]
				-\frac{126}{41}
			\end{bmatrix}& \notag \\
		x_{3} &= -\frac{41}{308}*\frac{126}{41} = -\frac{5166}{12628} = -\frac{9}{22}&
	\end{align}
	\begin{align}
		x_{2} &= \frac{-\frac{5}{4} + \frac{261}{176}}{\frac{41}{8}}& \notag \\
		&= \frac{261-220}{176}*\frac{8}{41}& \notag \\
		&= \frac{41}{176}*\frac{8}{41}& \notag \\
		&= \frac{328}{7216} = \frac{1}{22}& \\
		x_{1} &= \frac{6 - \frac{5}{22} + \frac{9}{22}}{8}& \notag \\
		&= \frac{\frac{132+4}{22}}{8}& \notag \\
		&= \frac{\frac{136}{22}}{8}& \notag \\
		&= \frac{136}{176} = \frac{17}{22}& \notag \\
	\label{eq:51x}
	\end{align}	