\section{Vector Norms}

	\subsection{Question (a)}

	\begin{align}
		x &= \begin{bmatrix}
			3 \\[0.3em]
			-5 \\[0.3em]
			\sqrt{2}
		\end{bmatrix}& \\
		|x|_{1} &= 3 - 5 + \sqrt{2} = -0.58579& \\
		|x|_{2} &= \sqrt{3^{2} + (-5)^{2} + (\sqrt{2})^{2}} = \sqrt{9 + 25 + 2} = \sqrt{36} = 6& \\
		|x|_{\infty} &= 5&
	\label{eq:64a}
	\end{align}

	\subsection{Question (b)}

	\begin{align}
		x &= \begin{bmatrix}
			e \\[0.3em]
			\pi \\[0.3em]
			2\sqrt{3}
		\end{bmatrix}& \\
		|x|_{1} &= e + \pi + 2\sqrt{3} = 9.3240& \\
		|x|_{2} &= \sqrt{e^{2} + \pi^{2} + (2\sqrt{3})^{2}} = \sqrt{e^{2} + \pi^{2} + 12} = \sqrt{29.259} = 5.4091& \\
		|x|_{\infty} &= 2\sqrt(3)&
	\label{eq:64b}
	\end{align}

	\subsection{Question (c)}

	\begin{align}
		x &= \begin{bmatrix}
			-3 \\[0.3em]
			2 \\[0.3em]
			-4 \\[0.3em]
			8 \\[0.3em]
			-1
		\end{bmatrix}& \\
		|x|_{1} &= -3 + 2 -4 +8 -1 = 2& \\
		|x|_{2} &= \sqrt{(-3)^{2} + 2^{2} + (-4)^{2} + 8^{2} (-1)^{2}} = \sqrt{9 + 4 + 16 + 64 + 1}& \notag \\
		&= \sqrt{94} = 9.6954& \\
		|x|_{\infty} &= 8&
	\label{eq:64c}
	\end{align}