\section{NOV24}
	\subsection{Higher Order IVP's (Linear)}
		\begin{align}
			a_{n}(x) \frac{d^{n}y}{dx^{n}} + a_{n-1}(x) \frac{d^{n-1}y}{dx^{n-1}} + a_{1}\frac{dy}{dx} + a_{0}y = f(x)
		\end{align}

		\begin{align}
			&y(x_{0}) = b_{0}&
			&y'(x_{0}) = b_{1}&
			&\dots&
			&y^{(n-1)}(x_{0}) = b_{n-1}&
		\end{align}

		\begin{itemize}
			\item{Taylor Polynomials:}
		\end{itemize}

		\begin{align}
			&xy'' - y' + 2y = x&
			&y(1) = 1&
			&y'(1)= 2&
		\end{align}

		To find the $4^{\text{th}}$-degree Taylor polynomial centered at $x=1$:
		Solve for $y''$:
		\begin{align}
			xy'' &= x + y' -2y'& \\
			y'' &= \frac{x+y'-2y}{x} = 1 + y'x^{-1} -2yx^{-1}& \\
			&= 1 + x^{-1}(y'-2y)& \\
			y''' &= -2x^{-2}(y'-2y) + x^{-1}(y''-2y')& \\
			y^{(4)} &= 4x^{-3}(y'-2y) - 2x^{-2}(y''-2y') - x^{-2}(y''-2y') + x^{-1}(y''' - 2y'')& \\
			&= 4x^{-3}(y'-2y) - 3x^{-2}(y''-2y') + x^{-1}(y''' - 2y'')&
		\end{align}

		\begin{align}
			y(1) = 1, y'(1) = 2, y''(1) = 1 + \frac{y'(1)-2y(1)}{1} = \frac{1+2-2}{1}=1 \\
			y'''(1) = -2(2-2) + 1(1-2(2)) = -3 \\
			y^{(4)} = 4(2 - 2) - 3(1-4) + 1(-3-2(1)) = 9 - 5 = 4
		\end{align}
		\begin{align}
			p_{4}(x) &= y(1) + y'(1)(x-1) + \frac{y''(1)}{2!}(x-1)^{2} + \frac{y'''(1)}{3!}(x-1)^{3}  + \frac{y^{(4)}(1)}{4!}(x-1)^{4}& \\
			&= 1 + 2(x-1) + \frac{1}{2}(x-1)^{2} + \frac{1}{2}(x-1)^{3}  + \frac{1}{6}(x-1)^{4}&
		\end{align}

		\begin{itemize}
			\item{Reducing a higher-order DE to a first-order system}
		\end{itemize}

		\begin{align}
			xy'' - y' + 2y &= x&
		\end{align}

		In normal form:

		\begin{align}
			y'' = 1 + y'x^{-1} -2yx^{-1}
		\end{align}

		For each derivative on the right-hand side of the normal form, make the substitution $u_{i} = y^{(i)}$:
		\begin{align}
			u_{1} &= y'&
		\end{align}

		Differentiate each substitution:
		\begin{align}
			u_{1}' &= y''&
		\end{align}

		\begin{align}
			y' &= u_{1}& \\
			u_{1}' &= 1 + u_{1}x^{-1} - 2yx^{-1}& \\
		\end{align}

		\begin{align}
			&y(1) = 1&
			&u_{1}(1) = 2&
		\end{align}

		Euler

		\begin{align}
			y_{n+1} &= y_{n} + h(u_{1n})& \\
			u_{n+1} &= u_{n} + h(1 + u_{1n}x_{n}^{-1}-2y_{n}x_{n}^{-1})&
		\end{align}

		\begin{table}[H]
			\begin{tabular}{|c|c|c|}
				\hline
				$x$ & $u_{1}$ & $y$ \\ \hline
				1 & 2 & 1 \hline
			\end{tabular}
		\end{table}

		Example:

		\begin{align}
			y^{(4)} - 2xy''' + y'' - y' + y &= 2x& \\
			y^{(4)} &= 2xy''' - y'' - y' + y&
		\end{align}

		\begin{align}
			&u_{1} = y'& &u_{1}' = y'' = u_{2}& \\
			&u_{2} = y''& &u_{2}' = y''' = u_{3}& \\
			&u_{3} = y'''& &u_{3}' = y^{(4)}&
		\end{align}

		\begin{align}
			&y' = u_{1}& &y(0) = 2& \\
			&u_{1}' = u_{2}& &u_{1}(0) = -1 \\
			&u_{2}' = u_{3}& &u_{2}(0) = 1&\\
			&u_{3}' = 2xu_{3} - u_[2] + u_{1} - y + 2x& &u_{3}(0) = 2&
		\end{align}
