\section{Picard Iterate}
	\begin{align}
		y_{n+1} &= y_{0} + \int_{x_{0}}^{x} f(t,y_{n}(t)) \ dt&
	\end{align}

	\subsection{Question (a)}
		\begin{align}
			&y' = x^{2} - 2y^{2} + 1&
			&y(0) = 0&
			&y_{2}(x)&
		\end{align}

		\begin{align}
			y_{n+1}(x) &= \int_{0}^{x} t^{2} - 2y_{n}(t)^{2} + 1 \ dt& \\
			&= \int_{0}^{x} t^{2} \ dt - \int_{0}^{x} 2y_{n}(t)^{2} \ dt + \int_{0}^{x} 1 \ dt& \notag \\
			&= \left[ \frac{t^{3}}{3} \right]_{0}^{x} - \int_{0}^{x} 2y_{n}(t)^{2} \ dt + [t]_{0}^{x}& \notag \\
			&= \frac{x^{3}}{3} - \int_{0}^{x} 2y_{n}(t)^{2} \ dt + x& \\
			y_{1}(x) &= \frac{x^{3}}{3} - \int_{0}^{x} 2y_{0}(t)^{2} \ dt + x& \\
			&= \frac{x^{3}}{3} + x&
		\end{align}

		\begin{align}
			y_{2}(x) &= \frac{x^{3}}{3} - \int_{0}^{x} 2y_{1}(t)^{2} \ dt + x& \\
			&= \frac{x^{3}}{3} - \int_{0}^{x} 2\left(\frac{t^{3}}{3} + t\right)^{2} \ dt + x& \notag \\
			&= \frac{x^{3}}{3} - \int_{0}^{x} 2\left(\frac{t^{6}}{9} + \frac{2t^{4}}{3} + t^{2}\right) \ dt + x& \notag \\
			&= \frac{x^{3}}{3} - 2\int_{0}^{x} \frac{t^{6}}{9} + \frac{2t^{4}}{3} + t^{2} \ dt + x& \notag \\
			&= \frac{x^{3}}{3} - 2\left[\frac{t^{7}}{63} + \frac{2t^{5}}{15} + \frac{t^{3}}{3}\right]_{0}^{x} + x& \notag \\
			&= \frac{x^{3}}{3} - \frac{2x^{7}}{63} - \frac{4x^{5}}{15} - \frac{2x^{3}}{3} + x& \notag \\
			&= - \frac{2x^{7}}{63} - \frac{4x^{5}}{15} - \frac{x^{3}}{3} + x&
		\end{align}

	\subsection{Question (b)}
		\begin{align}
			&\frac{dy}{dx} = 2e^{x} + y&
			&y(0) = 1&
			&y_{3}(x)&
		\end{align}

		\begin{align}
			y_{n+1}(x) &= 1 + \int_{0}^{x} 2e^{t} + y_{n}(t) \ dt& \\
			&= 1 + 2\int_{0}^{x} e^{t} \ dt + \int_{0}^{x} y_{n}(t) \ dt& \notag \\
			&= 1 + 2\left[e^{t}\right]_{0}^{x} + \int_{0}^{x} y_{n}(t) \ dt& \notag \\
			&= 1 + 2e^{x} + \int_{0}^{x} y_{n}(t) \ dt& \\
			y_{1}(x) &= 1 + 2e^{x} + \int_{0}^{x} y_{0}(t) \ dt& \\
			&= 1 + 2e^{x} + \int_{0}^{x} 1 \ dt& \notag \\
			&= 1 + 2e^{x} +  \left[t\right]_{0}^{x}& \notag \\
			&= 1 + 2e^{x} + x&
		\end{align}

		\begin{align}
			y_{2}(x) &= 1 + 2e^{x} + \int_{0}^{x} y_{1}(t) \ dt& \\
			&= 1 + 2e^{x} + \int_{0}^{x} 1 + 2e^{t} + t \ dt& \notag \\
			&= 1 + 2e^{x} + \left[t + 2e^{t} + \frac{t^{2}}{2}\right]_{0}^{x}& \notag \\
			&= 1 + 2e^{x} + x + 2e^{x} + \frac{x^{2}}{2}& \notag \\
			&= 4e^{x} + \frac{x^{2}}{2} + x + 1& \\
			y_{3}(x) &= 1 + 2e^{x} + \int_{0}^{x} y_{2}(t) \ dt& \\
			&= 1 + 2e^{x} + \int_{0}^{x} 4e^{t} + \frac{t^{2}}{2} + t + 1 \ dt& \notag \\
			&= 1 + 2e^{x} + \left[4e^{t} + \frac{t^{3}}{6} + \frac{t^{2}}{2} + t\right]_{0}^{x}& \notag \\
			&= 1 + 2e^{x} + 4e^{x} + \frac{x^{3}}{6} + \frac{x^{2}}{2} + x& \notag \\
			&= 6e^{x} + \frac{x^{3}}{6} + \frac{x^{2}}{2} + x + 1&
		\end{align}
