\section{Linear System Root Approximations}

	\subsection{Jacobi Method}
		\begin{align}
				x_{i} &= \frac{b_{i}-\sum_{j=1}^{i-1}a_{ij}x_{i} - \sum_{j=i+1}^{n}a_{ij}x_{i}}{a_{ii}}&,a_{ii}\neq0
		\end{align}

		\begin{align}
			\vec{x} &= -D^{-1}(L+U)\vec{x} + D^{-1}\vec{b}& \\
			T &= -D^{-1}(L+U)& \\
			\vec{c} &= D^{-1}\vec{b}& \\
			\vec{x} &= T\vec{x} + \vec{c}
		\end{align}

	\subsection{Gauss-Seidel}
		\begin{align}
			x_{i}^{(k+1)} &= \frac{b_{i}-\sum_{j=1}^{i-1}a_{ij}x_{i}^{k+1} - \sum_{j=i+1}^{n}a_{ij}x_{i}^{(k)}}{a_{ii}}&,a_{ii}\neq0
		\end{align}

		\begin{align}
			\vec{x} &= -(L+D)^{-1}U\vec{x} + (L+D)^{-1}\vec{b}& \\
			T &= (L+D)^{-1}U& \\
			\vec{c} &= (L+D)^{-1}\vec{b}& \\
			\vec{x} &= T\vec{x} + \vec{c}
		\end{align}

	\subsection{Criteria for Convergence}
		\begin{align}
			\vec{x}^{(k+1)} &= T\vec{x}^{(k)} + \vec{c}&, ||T|| < 1
		\end{align}

	\subsection{Error-Bound for Absolute Error}
		\begin{align}
			||\vec{x}-\vec{x}^{(k)}|| &\leq ||T||^{k}||\vec{x}^{(0)}-\vec{x}||& \\
			\frac{||\vec{x}-\vec{x}^{(k)}||}{||\vec{x}^{(0)}-\vec{x}||} &\leq ||T||^{k}& \notag \\
			\log{\left(\frac{||\vec{x}-\vec{x}^{(k)}||}{||\vec{x}^{(0)}-\vec{x}||}\right)} &\leq k \log{(||T||)}& \notag \\
			k &\geq \frac{\log{\left(\frac{||\vec{x}-\vec{x}^{(k)}||}{||\vec{x}^{(0)}-\vec{x}||}\right)}}{\log{(||T||)}}& \notag \\
			\lceil k \rceil &= \frac{\log{\left(\frac{||\vec{x}-\vec{x}^{(k)}||}{||\vec{x}^{(0)}-\vec{x}||}\right)}}{\log{\left(||T||\right)}}&
		\end{align}

		\begin{align}
			||\vec{x}-\vec{x}^{(k)}|| &\leq \frac{||T||^{k}}{1-||T||}||\vec{x}^{(1)}-\vec{x}^{(0)}||& \\
			\frac{||\vec{x}-\vec{x}^{(k)}||(1-||T||)}{||\vec{x}^{(1)}-\vec{x}^{(0)}||} &\leq ||T||^{k}& \notag \\
			\log{\left(\frac{||\vec{x}-\vec{x}^{(k)}||(1-||T||)}{||\vec{x}^{(1)}-\vec{x}^{(0)}||}\right)} &\leq k \log{\left(||T||\right)}& \notag \\
			k &\geq \frac{\log{\left(\frac{||\vec{x}-\vec{x}^{(k)}||(1-||T||)}{||\vec{x}^{(1)}-\vec{x}^{(0)}||}\right)}}{\log{\left(||T||\right)}}& \notag \\
			\lceil k \rceil &= \frac{\log{\left(\frac{||\vec{x}-\vec{x}^{(k)}||(1-||T||)}{||\vec{x}^{(1)}-\vec{x}^{(0)}||}\right)}}{\log{\left(||T||\right)}}& \notag \\
		\end{align}
